Qdt/Incremental/Query.lean
@@ -134,12 +134,38 @@ instance {i} : Hashable (InputVal i) := by
 instance {i} : Hashable (InputV i) :=
   inferInstanceAs (Hashable (Option (InputVal i)))
 
+def Key.rank : Key → Nat
+  | .moduleFile _ => 0
+  | .cst _ => 1
+  | .astSourceMap _ => 2
+  | .ast _ => 3
+  | .sourceMap _ => 3
+  | .imports _ => 4
+  | .declarationIndex _ => 4
+  | .transitiveImports _ => 5
+  | .declAst _ _ => 5
+  | .elabCmdAt _ _ => 6
+  | .elabDecl _ _ => 7
+  | .lookup _ _ => 8
+  | .lookupInfo _ _ => 8
+  | .constant _ _ => 9
+  | .type _ _ => 10
+  | .eval _ _ _ => 10
+  | .checkFile _ => 11
+  | .checkProject => 12
+
+def Key.rel (q q₀ : Key) : Prop :=
+  q.rank < q₀.rank
+
+theorem Key.rel_wf : WellFounded Key.rel :=
+  InvImage.wf Key.rank Nat.lt_wfRel.wf
+
 abbrev config : Incremental.BuildConfig where
   I := InputKey
   V := InputV
   Q := Key
   R := Val
-  rel := sorry
-  wf := sorry
+  rel := Key.rel
+  wf := Key.rel_wf
 
 end Qdt
