Incremental/ShakeC.lean
@@ -1,6 +1,6 @@
 module
 
-public import Incremental.Shake
+public import Incremental.ShakeStore
 
 namespace Incremental
 
@@ -12,23 +12,33 @@ variable
   [BEq ℭ.I] [LawfulBEq ℭ.I] [Hashable ℭ.I] [∀ i, Hashable (ℭ.V i)]
   [BEq ℭ.Q] [LawfulBEq ℭ.Q] [Hashable ℭ.Q] [∀ q, Hashable (ℭ.R q)]
 
+instance {ℭ : BuildConfig} {J : Type}
+    [BEq ℭ.I] [Hashable ℭ.I] [∀ i, Hashable (ℭ.V i)]
+    [BEq ℭ.Q] [Hashable ℭ.Q] [∀ q, Hashable (ℭ.R q)]
+    [Input ℭ J] :
+    Nonempty (Tasks Monad ℭ → ∀ q, ShakeRT.Store ℭ J → ℭ.R q × ShakeRT.Store ℭ J) :=
+  ⟨sorry⟩
+
 @[extern "lean_shake_build"]
-public unsafe opaque shakeCBuild
+public opaque shakeCBuild
     {ℭ : BuildConfig} {J : Type}
     [BEq ℭ.I] [Hashable ℭ.I] [∀ i, Hashable (ℭ.V i)]
     [BEq ℭ.Q] [Hashable ℭ.Q] [∀ q, Hashable (ℭ.R q)]
     [Input ℭ J] :
     Tasks Monad ℭ → ∀ q,
-    Shake.Store ℭ J → ℭ.R q × Shake.Store ℭ J
+    ShakeRT.Store ℭ J → ℭ.R q × ShakeRT.Store ℭ J
 
-@[expose] public unsafe def ShakeC : Build Monad ℭ J where
-  σ := Shake.Store ℭ J
+public def ShakeC : Build Monad ℭ J where
+  cId := inferInstance
+  σ := ShakeRT.Store ℭ J
   init inputs := {
     inputs
     memos := DHashMap.emptyWithCapacity 4096
   }
   inputs store := Input.get store.inputs
   set i v := modify fun store => { store with inputs := Input.set store.inputs i v }
-  build := shakeCBuild
+  build tasks q store :=
+    let (r, s) := shakeCBuild tasks q store
+    (⟨r, sorry⟩, s)
 
 end Incremental
