Incremental/ShakeCPS.lean
@@ -1,6 +1,6 @@
 module
 
-public import Incremental.Shake
+public import Incremental.ShakeStore
 public import Mathlib.Control.Monad.Cont
 
 namespace Incremental
@@ -13,8 +13,9 @@ variable
   [BEq ℭ.I] [LawfulBEq ℭ.I] [Hashable ℭ.I] [∀ i, Hashable (ℭ.V i)]
   [BEq ℭ.Q] [LawfulBEq ℭ.Q] [Hashable ℭ.Q] [∀ q, Hashable (ℭ.R q)]
 
-public def ShakeCPS : Build Monad ℭ J where
-  σ := Shake.Store ℭ J
+@[expose] public def ShakeCPS : Build Monad ℭ J where
+  cId := inferInstance
+  σ := ShakeRT.Store ℭ J
   init inputs := {
     inputs
     memos := DHashMap.emptyWithCapacity 1024
@@ -22,7 +23,7 @@ public def ShakeCPS : Build Monad ℭ J where
   inputs store := Input.get store.inputs
   set i v := modify fun store =>
     { store with inputs := Input.set store.inputs i v }
-  build tasks q₀ := fun store =>
+  build tasks q₀ store :=
     let ι₀ := Input.get store.inputs
     runST fun σ => do
       let memos ← ST.mkRef (σ := σ) store.memos
@@ -47,8 +48,8 @@ public def ShakeCPS : Build Monad ℭ J where
                 deps.modify (·.insert q h)
               ki v
           let recompute : ST σ (ℭ.R q₀) :=
-            (tasks ι₀ q (ContT (ℭ.R q₀) (ST σ)) input' (fun q₁ _hq => fetch' q₁)).run fun value => do
-              let m : Shake.Memo ℭ q := { value, deps := ← deps.get, inputDeps := ← inputDeps.get }
+            (tasks q (ContT (ℭ.R q₀) (ST σ)) input' (fun q₁ _hq => fetch' q₁)).run fun value => do
+              let m : ShakeRT.Memo ℭ q := { value, deps := ← deps.get, inputDeps := ← inputDeps.get }
               started.modify (·.insert q m)
               memos.modify (·.insert q m)
               k value
@@ -69,8 +70,8 @@ public def ShakeCPS : Build Monad ℭ J where
                   if h != oldHash then recompute
                   else cont
           | none => recompute
-      termination_by (ℭ.wf ι₀).wrap q
+      termination_by ℭ.wf.wrap q
       decreasing_by all_goals sorry
-      return (← (fetch q₀).run pure, ⟨store.inputs, ← memos.get⟩)
+      return (⟨← (fetch q₀).run pure, sorry⟩, ⟨store.inputs, ← memos.get⟩)
 
 end Incremental
