Incremental/ShakeStore.lean
@@ -1,0 +1,30 @@
+module
+
+public import Incremental.Basic
+
+@[expose] public section
+
+namespace Incremental
+
+open Std (DHashMap HashMap)
+
+variable (ℭ : BuildConfig)
+  [BEq ℭ.I] [Hashable ℭ.I]
+  [BEq ℭ.Q] [Hashable ℭ.Q] [∀ q, Hashable (ℭ.R q)]
+
+namespace ShakeRT
+
+structure Memo (q₀ : ℭ.Q) where
+  value : ℭ.R q₀
+  deps : HashMap ℭ.Q UInt64
+  inputDeps : HashMap ℭ.I UInt64
+  hash : UInt64 := hash value
+  hash_value : Hashable.hash value = hash := by rfl
+
+structure Store (J : Type) where
+  inputs : J
+  memos : DHashMap ℭ.Q (ShakeRT.Memo ℭ)
+
+end ShakeRT
+
+end Incremental
