Qdt/Control.lean
@@ -14,7 +14,7 @@ open System (FilePath)
 
 open Std (HashMap HashSet)
 
-variable (ι₀ : ∀ i, config.V i) (q₀ : config.Q)
+variable (q₀ : config.Q)
 
 structure ElabContext where
   filepath : FilePath
@@ -36,52 +36,52 @@ structure ElabState where
 deriving Inhabited
 
 abbrev ElabM :=
-  Task Monad config ι₀ q₀
+  Task Monad config q₀
   |> StateT ElabState
   |> ReaderT ElabContext
 
-abbrev TermM (n : Nat) := ReaderT (TermContext n) (ElabM ι₀ q₀)
-abbrev SemM (n c : Nat) := ReaderT (Env n c) (ElabM ι₀ q₀)
+abbrev TermM (n : Nat) := ReaderT (TermContext n) (ElabM q₀)
+abbrev SemM (n c : Nat) := ReaderT (Env n c) (ElabM q₀)
 
-instance {n} : MonadLiftT (SemM ι₀ q₀ n n) (TermM ι₀ q₀ n) where
+instance {n} : MonadLiftT (SemM q₀ n n) (TermM q₀ n) where
   monadLift m n := m n.env
 
-@[inline] def currentDecl : ElabM ι₀ q₀ Name := do
+@[inline] def currentDecl : ElabM q₀ Name := do
   return (← read).currentDecl
 
-@[inline] def currentPath : ElabM ι₀ q₀ Path := do
+@[inline] def currentPath : ElabM q₀ Path := do
   return (← read).path
 
-@[inline] def withChild {α : Type} (i : Nat) : ElabM ι₀ q₀ α → ElabM ι₀ q₀ α :=
+@[inline] def withChild {α : Type} (i : Nat) : ElabM q₀ α → ElabM q₀ α :=
   ReaderT.adapt fun ctx => { ctx with path := i :: ctx.path }
 
-@[inline] def getUnivParams : ElabM ι₀ q₀ (List Name) := do
+@[inline] def getUnivParams : ElabM q₀ (List Name) := do
   return (← read).univParams
 
-@[inline] def emitDiagnostic (err : Error) : ElabM ι₀ q₀ Unit := do
-  let path ← currentPath ι₀ q₀
+@[inline] def emitDiagnostic (err : Error) : ElabM q₀ Unit := do
+  let path ← currentPath q₀
   modify fun st => { st with diagnostics := st.diagnostics.push { path, error := err } }
 
-def raiseError {α : Type} (err : Error) : OptionT (ElabM ι₀ q₀) α := do
-  emitDiagnostic ι₀ q₀ err
+def raiseError {α : Type} (err : Error) : OptionT (ElabM q₀) α := do
+  emitDiagnostic q₀ err
   failure
 
-@[inline] def emitHover (hover : HoverContent) : ElabM ι₀ q₀ Unit := do
+@[inline] def emitHover (hover : HoverContent) : ElabM q₀ Unit := do
   if !(← readThe ElabContext).collectHovers then return
-  let path ← currentPath ι₀ q₀
+  let path ← currentPath q₀
   modify fun st => { st with hovers := st.hovers.push { path, hover } }
 
-def getLocalEnv : ElabM ι₀ q₀ Global := do
+def getLocalEnv : ElabM q₀ Global := do
   return (← get).localEnv
 
-def fetchConstant (name : Name) : ElabM ι₀ q₀ (Option Constant) := do
+def fetchConstant (name : Name) : ElabM q₀ (Option Constant) := do
   let st ← get
   if let some e := st.localEnv[name]? then
     return some e
   let ctx ← readThe ElabContext
   if let some result := st.entryCache[name]? then
     return result
-  let (declIndex, _) ← (Task.fetch (c := Monad) (ℭ := config) (ι₀ := ι₀) (q₀ := q₀) (Key.declarationIndex ctx.filepath) sorry : Task Monad config ι₀ q₀ _)
+  let (declIndex, _) ← (Task.fetch (c := Monad) (ℭ := config) (q₀ := q₀) (Key.declarationIndex ctx.filepath) sorry : Task Monad config q₀ _)
   let currentDeclName := (← read).currentDecl
   if let some idx := declIndex[name]? then
     if let some currentIdx := declIndex[currentDeclName]? then
@@ -89,64 +89,64 @@ def fetchConstant (name : Name) : ElabM ι₀ q₀ (Option Constant) := do
         modify fun st => { st with entryCache := st.entryCache.insert name none }
         return none
   let result : Val (Key.constant ctx.filepath name) ←
-    (Task.fetch (c := Monad) (ℭ := config) (ι₀ := ι₀) (q₀ := q₀) (Key.constant ctx.filepath name) sorry : Task Monad config ι₀ q₀ _)
+    (Task.fetch (c := Monad) (ℭ := config) (q₀ := q₀) (Key.constant ctx.filepath name) sorry : Task Monad config q₀ _)
   let result : Option Constant := result.map Prod.fst
   modify fun st => { st with entryCache := st.entryCache.insert name result }
   return result
 
-def fetchConstantInfo (name : Name) : ElabM ι₀ q₀ (Option ConstantInfo) := do
-  let some e ← fetchConstant ι₀ q₀ name | return none
+def fetchConstantInfo (name : Name) : ElabM q₀ (Option ConstantInfo) := do
+  let some e ← fetchConstant q₀ name | return none
   return some (match e with
     | .definition info | .opaque info | .axiom info
     | .recursor info | .constructor info | .inductive info => info.toConstantInfo)
 
-def fetchDefinition (name : Name) : ElabM ι₀ q₀ (Option (Tm 0)) := do
-  let some (.definition info) ← fetchConstant ι₀ q₀ name | return none
+def fetchDefinition (name : Name) : ElabM q₀ (Option (Tm 0)) := do
+  let some (.definition info) ← fetchConstant q₀ name | return none
   return some info.tm
 
-def fetchInductive (name : Name) : ElabM ι₀ q₀ (Option InductiveInfo) := do
-  let some (.inductive info) ← fetchConstant ι₀ q₀ name | return none
+def fetchInductive (name : Name) : ElabM q₀ (Option InductiveInfo) := do
+  let some (.inductive info) ← fetchConstant q₀ name | return none
   return some info
 
-def fetchRecursor (name : Name) : ElabM ι₀ q₀ (Option RecursorInfo) := do
-  let some (.recursor info) ← fetchConstant ι₀ q₀ name | return none
+def fetchRecursor (name : Name) : ElabM q₀ (Option RecursorInfo) := do
+  let some (.recursor info) ← fetchConstant q₀ name | return none
   return some info
 
-def fetchConstructor (name : Name) : ElabM ι₀ q₀ (Option ConstructorInfo) := do
-  let some (.constructor info) ← fetchConstant ι₀ q₀ name | return none
+def fetchConstructor (name : Name) : ElabM q₀ (Option ConstructorInfo) := do
+  let some (.constructor info) ← fetchConstant q₀ name | return none
   return some info
 
-def addConstant (name : Name) (constant : Constant) : ElabM ι₀ q₀ Bool := do
+def addConstant (name : Name) (constant : Constant) : ElabM q₀ Bool := do
   let st ← get
   if name ∈ st.localEnv then
-    emitDiagnostic ι₀ q₀ (.alreadyDefined name)
+    emitDiagnostic q₀ (.alreadyDefined name)
     return false
   let ctx ← readThe ElabContext
   let currentDeclName := (← read).currentDecl
-  let (declIndex, _) ← (fetch (q₀ := q₀) (Key.declarationIndex ctx.filepath) sorry : Task Monad config ι₀ q₀ _)
+  let (declIndex, _) ← (fetch (q₀ := q₀) (Key.declarationIndex ctx.filepath) sorry : Task Monad config q₀ _)
   match declIndex[name]? with
   | some nameIdx =>
       match declIndex[currentDeclName]? with
       | some currentIdx =>
           if nameIdx != currentIdx then
-            emitDiagnostic ι₀ q₀ (.alreadyDefined name)
+            emitDiagnostic q₀ (.alreadyDefined name)
             return false
       | none => pure ()
   | none =>
       let existing : Val (Key.constant ctx.filepath name) ←
-        (fetch (q₀ := q₀) (Key.constant ctx.filepath name) sorry : Task Monad config ι₀ q₀ _)
+        (fetch (q₀ := q₀) (Key.constant ctx.filepath name) sorry : Task Monad config q₀ _)
       if existing.isSome then
-        emitDiagnostic ι₀ q₀ (.alreadyDefined name)
+        emitDiagnostic q₀ (.alreadyDefined name)
         return false
   set { st with localEnv := st.localEnv.insert name constant }
   return true
 
-def replaceEntry (name : Name) (constant : Constant) : ElabM ι₀ q₀ Unit := do
+def replaceEntry (name : Name) (constant : Constant) : ElabM q₀ Unit := do
   let st ← get
   set { st with localEnv := st.localEnv.insert name constant }
 
-def ElabM.run {α : Type} (ctx : ElabContext) (action : ElabM ι₀ q₀ α) :
-    Task Monad config ι₀ q₀ (α × Global × ElabInfo) := do
+def ElabM.run {α : Type} (ctx : ElabContext) (action : ElabM q₀ α) :
+    Task Monad config q₀ (α × Global × ElabInfo) := do
   let state : ElabState := {
     localEnv := ∅
     sorryId := 0
