Qdt/Conversion.lean
@@ -6,7 +6,7 @@ public section
 
 namespace Qdt
 
-variable (ι₀ : ∀ i, InputV i) (q₀ : Key)
+variable (q₀ : Key)
 
 inductive ConvState where
   | rigid
@@ -15,7 +15,7 @@ inductive ConvState where
 
 mutual
 
-public partial def VTm.conv {n} (a b : VTm n) (cs : ConvState := .rigid) : ElabM ι₀ q₀ Bool :=
+public partial def VTm.conv {n} (a b : VTm n) (cs : ConvState := .rigid) : ElabM q₀ Bool :=
   match a, b with
   | .u' i₁, .u' i₂ => return i₁ == i₂
   | .glued ne₁ _ _, .glued ne₂ _ _ => do
@@ -23,62 +23,62 @@ public partial def VTm.conv {n} (a b : VTm n) (cs : ConvState := .rigid) : ElabM
       | .flex => ne₁.conv ne₂ cs
       | .rigid =>
         if ← ne₁.conv ne₂ .flex then return true
-        (← a.whnf ι₀ q₀).conv (← b.whnf ι₀ q₀) .full
-      | .full => (← a.whnf ι₀ q₀).conv (← b.whnf ι₀ q₀) cs
-  | .glued _ _ _, other => do (← a.whnf ι₀ q₀).conv other cs
-  | other, .glued _ _ _ => do other.conv (← b.whnf ι₀ q₀) cs
+        (← a.whnf q₀).conv (← b.whnf q₀) .full
+      | .full => (← a.whnf q₀).conv (← b.whnf q₀) cs
+  | .glued _ _ _, other => do (← a.whnf q₀).conv other cs
+  | other, .glued _ _ _ => do other.conv (← b.whnf q₀) cs
   | .neutral n₁, .neutral n₂ => do
       match cs with
       | .flex => n₁.conv n₂ cs
       | _ =>
-        let a' ← (VTm.neutral n₁).whnf ι₀ q₀
-        let b' ← (VTm.neutral n₂).whnf ι₀ q₀
+        let a' ← (VTm.neutral n₁).whnf q₀
+        let b' ← (VTm.neutral n₂).whnf q₀
         match a', b' with
         | .neutral n₁', .neutral n₂' => n₁'.conv n₂' cs
         | _, _ => a'.conv b' cs
   | .lam _ _ ⟨env₁, body₁⟩, .lam _ _ ⟨env₂, body₂⟩ => do
       let var : VTm (n + 1) := VTm.varAt n
-      let b₁Val ← body₁.eval ι₀ q₀ (env₁.weaken.cons var)
-      let b₂Val ← body₂.eval ι₀ q₀ (env₂.weaken.cons var)
+      let b₁Val ← body₁.eval q₀ (env₁.weaken.cons var)
+      let b₂Val ← body₂.eval q₀ (env₂.weaken.cons var)
       b₁Val.conv b₂Val cs
   | .lam _ _ ⟨env, body⟩, other => do
       let var : VTm (n + 1) := VTm.varAt n
-      let bVal ← body.eval ι₀ q₀ (env.weaken.cons var)
+      let bVal ← body.eval q₀ (env.weaken.cons var)
       match other.weaken (m := n + 1) with
       | .neutral ne =>
-          let oVal ← (VTm.neutral ne).app ι₀ q₀ var
+          let oVal ← (VTm.neutral ne).app q₀ var
           bVal.conv oVal cs
       | _ => return false
   | other, .lam _ _ ⟨env, body⟩ => do
       let var : VTm (n + 1) := VTm.varAt n
-      let bVal ← body.eval ι₀ q₀ (env.weaken.cons var)
+      let bVal ← body.eval q₀ (env.weaken.cons var)
       match other.weaken (m := n + 1) with
       | .neutral ne =>
-          let oVal ← (VTm.neutral ne).app ι₀ q₀ var
+          let oVal ← (VTm.neutral ne).app q₀ var
           oVal.conv bVal cs
       | _ => return false
   | .pi' _ a₁ ⟨env₁, b₁⟩, .pi' _ a₂ ⟨env₂, b₂⟩ => do
       if !(← a₁.conv a₂ cs) then return false
       let var : VTm (n + 1) := VTm.varAt n
-      let b₁Val ← b₁.eval ι₀ q₀ (env₁.weaken.cons var)
-      let b₂Val ← b₂.eval ι₀ q₀ (env₂.weaken.cons var)
+      let b₁Val ← b₁.eval q₀ (env₁.weaken.cons var)
+      let b₂Val ← b₂.eval q₀ (env₂.weaken.cons var)
       b₁Val.conv b₂Val cs
   | .neutral ne, other => do
-      match ← (VTm.neutral ne).whnf ι₀ q₀ with
+      match ← (VTm.neutral ne).whnf q₀ with
       | .neutral _ => return false
       | v => v.conv other cs
   | other, .neutral ne => do
-      match ← (VTm.neutral ne).whnf ι₀ q₀ with
+      match ← (VTm.neutral ne).whnf q₀ with
       | .neutral _ => return false
       | v => other.conv v cs
   | _, _ => return false
 
-partial def etaConv {n} (ne : Neutral n) (other : VTm n) (cs : ConvState) : ElabM ι₀ q₀ Bool := do
+partial def etaConv {n} (ne : Neutral n) (other : VTm n) (cs : ConvState) : ElabM q₀ Bool := do
   let ⟨.const ctorName _us, sp⟩ := ne
     | return false
-  let some ctorInfo ← fetchConstructor ι₀ q₀ ctorName
+  let some ctorInfo ← fetchConstructor q₀ ctorName
     | return false
-  let some indInfo ← fetchInductive ι₀ q₀ ctorInfo.indName
+  let some indInfo ← fetchInductive q₀ ctorInfo.indName
     | return false
   if indInfo.numIndices ≠ 0 ∨ indInfo.numMinors ≠ 1 then
     return false
@@ -88,11 +88,11 @@ partial def etaConv {n} (ne : Neutral n) (other : VTm n) (cs : ConvState) : Elab
     return false
   let fields := args.drop indInfo.numParams
   List.finRange fields.length |>.allM (fun (i : Fin fields.length) => do
-    let proj ← other.proj ι₀ q₀ i.val
+    let proj ← other.proj q₀ i.val
     proj.conv fields[i] cs
   )
 
-partial def Neutral.conv {n} : Neutral n → Neutral n → ConvState → ElabM ι₀ q₀ Bool
+partial def Neutral.conv {n} : Neutral n → Neutral n → ConvState → ElabM q₀ Bool
   | ne₁@⟨h₁, sp₁⟩, ne₂@⟨h₂, sp₂⟩, cs => do
       match h₁, h₂ with
       | .var v₁, .var v₂ =>
@@ -102,39 +102,39 @@ partial def Neutral.conv {n} : Neutral n → Neutral n → ConvState → ElabM �
             match cs with
             | .rigid =>
                 if ← sp₁.conv sp₂ .flex then return true
-                match ← deltaReduction ι₀ q₀ n₁ us₁ with
-                | some v₁ => (← applySpine ι₀ q₀ sp₁ v₁).conv (← applySpine ι₀ q₀ sp₂ v₁) .full
+                match ← deltaReduction q₀ n₁ us₁ with
+                | some v₁ => (← applySpine q₀ sp₁ v₁).conv (← applySpine q₀ sp₂ v₁) .full
                 | none => sp₁.conv sp₂ .full
             | _ => sp₁.conv sp₂ cs
           else
             match cs with
             | .flex => return false
             | _ =>
-              match ← deltaReduction ι₀ q₀ n₁ us₁, ← deltaReduction ι₀ q₀ n₂ us₂ with
+              match ← deltaReduction q₀ n₁ us₁, ← deltaReduction q₀ n₂ us₂ with
               | some v₁, some v₂ =>
-                  (← applySpine ι₀ q₀ sp₁ v₁).conv (← applySpine ι₀ q₀ sp₂ v₂) .full
+                  (← applySpine q₀ sp₁ v₁).conv (← applySpine q₀ sp₂ v₂) .full
               | some v₁, none =>
-                  (← applySpine ι₀ q₀ sp₁ v₁).conv (.neutral ne₂) .full
+                  (← applySpine q₀ sp₁ v₁).conv (.neutral ne₂) .full
               | none, some v₂ =>
-                  (VTm.neutral ne₁).conv (← applySpine ι₀ q₀ sp₂ v₂) .full
+                  (VTm.neutral ne₁).conv (← applySpine q₀ sp₂ v₂) .full
               | none, none =>
                   return (← etaConv ne₁ (.neutral ne₂) cs) || (← etaConv ne₂ (.neutral ne₁) cs)
       | .const n₁ us₁, .var _ =>
           match cs with
           | .flex => return false
           | _ =>
-            match ← deltaReduction ι₀ q₀ n₁ us₁ with
-            | some v₁ => (← applySpine ι₀ q₀ sp₁ v₁).conv (.neutral ne₂) .full
+            match ← deltaReduction q₀ n₁ us₁ with
+            | some v₁ => (← applySpine q₀ sp₁ v₁).conv (.neutral ne₂) .full
             | none => etaConv ne₁ (.neutral ne₂) cs
       | .var _, .const n₂ us₂ =>
           match cs with
           | .flex => return false
           | _ =>
-            match ← deltaReduction ι₀ q₀ n₂ us₂ with
-            | some v₂ => (VTm.neutral ne₁).conv (← applySpine ι₀ q₀ sp₂ v₂) .full
+            match ← deltaReduction q₀ n₂ us₂ with
+            | some v₂ => (VTm.neutral ne₁).conv (← applySpine q₀ sp₂ v₂) .full
             | none => etaConv ne₂ (.neutral ne₁) cs
 
-partial def Spine.conv {n} : Spine n → Spine n → ConvState → ElabM ι₀ q₀ Bool
+partial def Spine.conv {n} : Spine n → Spine n → ConvState → ElabM q₀ Bool
   | .nil, .nil, _ => return true
   | .app sp₁ t₁, .app sp₂ t₂, cs => return (← t₁.conv t₂ cs) && (← sp₁.conv sp₂ cs)
   | .proj sp₁ i₁, .proj sp₂ i₂, cs => return i₁ == i₂ && (← sp₁.conv sp₂ cs)
@@ -142,16 +142,16 @@ partial def Spine.conv {n} : Spine n → Spine n → ConvState → ElabM ι₀ q
 
 end
 
-public partial def VTy.conv {n} (a b : VTy n) (cs : ConvState := .rigid) : ElabM ι₀ q₀ Bool :=
+public partial def VTy.conv {n} (a b : VTy n) (cs : ConvState := .rigid) : ElabM q₀ Bool :=
   match a, b with
   | .u i₁, .u i₂ => return i₁ == i₂
   | .pi _ a₁ ⟨env₁, b₁⟩, .pi _ a₂ ⟨env₂, b₂⟩ => do
       if !(← a₁.conv a₂ cs) then return false
       let var : VTm (n + 1) := VTm.varAt n
-      let b₁Val ← b₁.eval ι₀ q₀ (env₁.weaken.cons var)
-      let b₂Val ← b₂.eval ι₀ q₀ (env₂.weaken.cons var)
+      let b₁Val ← b₁.eval q₀ (env₁.weaken.cons var)
+      let b₂Val ← b₂.eval q₀ (env₂.weaken.cons var)
       b₁Val.conv b₂Val cs
-  | .el n₁, .el n₂ => n₁.conv ι₀ q₀ n₂ cs
+  | .el n₁, .el n₂ => n₁.conv q₀ n₂ cs
   | _, _ => return false
 
 end Qdt
