Qdt/Params.lean
@@ -9,38 +9,38 @@ namespace Qdt
 open Lean (Name)
 open Frontend (Ast Path)
 
-variable (ι₀ : ∀ i, InputV i) (q₀ : Key)
+variable (q₀ : Key)
 
 def getTypedBinder : Ast → Option (Name × Ast)
   | .node `Binder.typed cs => some (cs[0]!.getName, cs[1]!)
   | _ => none
 
 public def Params.elabWithLevels {n : Nat} (ctx : TermContext n) (params : List Ast) :
-    OptionT (ElabM ι₀ q₀) (TermContext (n + params.length) × Ctx n (n + params.length) × List Universe) :=
+    OptionT (ElabM q₀) (TermContext (n + params.length) × Ctx n (n + params.length) × List Universe) :=
   Nat.zero_add params.length ▸ go n 0 ctx .nil [] params
   where
     go {a : Nat} (b : Nat) (idx : Nat) (ctx : TermContext b) (acc : Ctx a b) (levels : List Universe) :
       (params : List Ast) →
-        OptionT (ElabM ι₀ q₀) (TermContext (b + params.length) × Ctx a (b + params.length) × List Universe)
+        OptionT (ElabM q₀) (TermContext (b + params.length) × Ctx a (b + params.length) × List Universe)
     | [] => return (ctx, acc, levels.reverse)
     | ast :: bs => do
         let some (name, tyAst) := getTypedBinder ast
           | failure
-        let (ty, level) ← OptionT.lift (withChild ι₀ q₀ idx (withChild ι₀ q₀ 1 (checkTyWithLevel ι₀ q₀ ctx tyAst)))
-        let tyVal ← ty.eval ι₀ q₀ ctx.env
-        let tyQuoted ← tyVal.quote ι₀ q₀
-        withChild ι₀ q₀ idx (withChild ι₀ q₀ 0 (emitHover ι₀ q₀ (.localVar name ctx.names tyQuoted)))
+        let (ty, level) ← OptionT.lift (withChild q₀ idx (withChild q₀ 1 (checkTyWithLevel q₀ ctx tyAst)))
+        let tyVal ← ty.eval q₀ ctx.env
+        let tyQuoted ← tyVal.quote q₀
+        withChild q₀ idx (withChild q₀ 0 (emitHover q₀ (.localVar name ctx.names tyQuoted)))
         let ctx := ctx.bind name tyVal
         let ih ← go (b + 1) (idx + 1) ctx (acc.snoc ⟨name, ty⟩) (level :: levels) bs
         return by simpa only [List.length_cons, Nat.add_comm bs.length, Nat.add_assoc b] using ih
 
 public def Params.elabFrom {n : Nat} (ctx : TermContext n) (params : List Ast) :
-    OptionT (ElabM ι₀ q₀) (TermContext (n + params.length) × Ctx n (n + params.length)) := do
-  let (ctx, tele, _) ← Params.elabWithLevels ι₀ q₀ ctx params
+    OptionT (ElabM q₀) (TermContext (n + params.length) × Ctx n (n + params.length)) := do
+  let (ctx, tele, _) ← Params.elabWithLevels q₀ ctx params
   return (ctx, tele)
 
 public def Params.elab (params : List Ast) :
-    OptionT (ElabM ι₀ q₀) (TermContext params.length × Ctx 0 params.length) :=
-  Nat.zero_add params.length ▸ Params.elabFrom ι₀ q₀ TermContext.empty params
+    OptionT (ElabM q₀) (TermContext params.length × Ctx 0 params.length) :=
+  Nat.zero_add params.length ▸ Params.elabFrom q₀ TermContext.empty params
 
 end Qdt
