Qdt/Quote.lean
@@ -4,64 +4,64 @@ public import Qdt.Nbe
 
 namespace Qdt
 
-variable (ι₀ : ∀ i, InputV i) (q₀ : Key)
+variable (q₀ : Key)
 
 mutual
 
-public partial def VTy.quote {n} : VTy n → ElabM ι₀ q₀ (Ty n)
+public partial def VTy.quote {n} : VTy n → ElabM q₀ (Ty n)
   | .u i => return .u i
   | .pi x a ⟨env, b⟩ => do
       let a ← a.quote
-      let b ← b.eval ι₀ q₀ (env.weaken.cons (VTm.varAt n))
+      let b ← b.eval q₀ (env.weaken.cons (VTm.varAt n))
       let b ← b.quote
       return .pi x a b
   | .el n => return .el (← n.quote)
 
-public partial def VTm.quote {n} : VTm n → ElabM ι₀ q₀ (Tm n)
+public partial def VTm.quote {n} : VTm n → ElabM q₀ (Tm n)
   | .u' i => return .u' i
   | .neutral n => n.quote
   | .lam x a ⟨env, b⟩ => do
       let a ← a.quote
-      let b ← b.eval ι₀ q₀ (env.weaken.cons (VTm.varAt n))
+      let b ← b.eval q₀ (env.weaken.cons (VTm.varAt n))
       let b ← b.quote
       return .lam x a b
   | .pi' x a ⟨env, b⟩ => do
       let a ← a.quote
-      let b ← b.eval ι₀ q₀ (env.weaken.cons (VTm.varAt n))
+      let b ← b.eval q₀ (env.weaken.cons (VTm.varAt n))
       let b ← b.quote
       return .pi' x a b
   | .glued ne _ _ => ne.quote
 
-partial def Head.quote {n} : Head n → ElabM ι₀ q₀ (Tm n)
+partial def Head.quote {n} : Head n → ElabM q₀ (Tm n)
   | .var i => return .var i.rev
   | .const name us => return .const name us
 
-partial def Neutral.quote {n} (ne : Neutral n) : ElabM ι₀ q₀ (Tm n) := do
+partial def Neutral.quote {n} (ne : Neutral n) : ElabM q₀ (Tm n) := do
   let ⟨h, sp⟩ := ne
-  let rec go : Spine n → ElabM ι₀ q₀ (Tm n)
+  let rec go : Spine n → ElabM q₀ (Tm n)
     | .nil => h.quote
     | .app sp t => return .app (← go sp) (← t.quote)
     | .proj sp i => return .proj i (← go sp)
   go sp
 
-public partial def VTy.reify {n} : VTy n → ElabM ι₀ q₀ (Tm n)
+public partial def VTy.reify {n} : VTy n → ElabM q₀ (Tm n)
   | .u i => return .u' i
   | .pi x a ⟨env, b⟩ => do
       let a ← a.reify
-      let b ← b.eval ι₀ q₀ (env.weaken.cons (VTm.varAt n))
+      let b ← b.eval q₀ (env.weaken.cons (VTm.varAt n))
       let b ← b.reify
       return .pi' x a b
   | .el n => n.quote
 
-public partial def VTy.inferLevel {n} (ctx : VCtx n) : VTy n → ElabM ι₀ q₀ Universe
+public partial def VTy.inferLevel {n} (ctx : VCtx n) : VTy n → ElabM q₀ Universe
   | .u i => return i.mkSucc
   | .pi _x a ⟨env, b⟩ => do
       let aLevel ← a.inferLevel ctx
-      let bVal : VTy (n + 1) ← b.eval ι₀ q₀ (env.weaken.cons (VTm.varAt n))
+      let bVal : VTy (n + 1) ← b.eval q₀ (env.weaken.cons (VTm.varAt n))
       let bLevel ← bVal.inferLevel (ctx.snoc ⟨.anonymous, a⟩)
       return aLevel.mkMax bLevel
   | .el ⟨.const name us, _sp⟩ => do
-      let some info ← fetchConstantInfo ι₀ q₀ name
+      let some info ← fetchConstantInfo q₀ name
         | panic! s!"inferLevel: unknown constant {name}"
       let ty := info.ty.substLevels (info.univParams.zip us)
       let some u := ty.getResultUniverse?
